\documentclass{article}
\usepackage[utf8]{inputenc}
\usepackage{amsmath}

\begin{document}


\begin{equation*}
        V=V(x_0,x_0)+\sum_{s=1}^{M}\sum_{i=1}^{N_s}\lambda_{si}(V(x_0,x_{si})+V(x_{si},x_{si}))
        +\sum_{s=1}^{M}\sum_{i=1}^{N_s}\sum_{t=s+1}^{M}\sum_{j=1}^{N_t}\lambda_{si}\lambda_{tj}V(x_{si},x_{tj})
        +V_{bias}(\{\lambda\})
  \label{eqn:V_msld}
\end{equation*}

\begin{equation*}
        V_{bias}(\{\lambda\})=V_{fixed}(\{\lambda\})+V_{quadratic}(\{\lambda\})
        +V_{end}(\{\lambda\})+V_{skew}(\{\lambda\})
  \label{eqn:V_bias}
\end{equation*}

\begin{equation*}
	V_{fixed}(\{\lambda\})= \begin{cases}
		0 & \text{if reference state} \\
		\lambda(\Delta G_{model}+2.303RT(pK_a-pH)) & \text{otherwise}
	\end{cases}
  \label{eqn:V_fixed}
\end{equation*}

\end{document}
